```{=latex} 
\begin{equation}
f(y) = 
\begin{cases} 
\frac{1} {\Gamma(\frac{\mu}{\beta}) \beta^{\frac{\mu}{\beta}}} {(y - \epsilon)}^{\frac{\mu}{\beta} - 1} \exp(- \frac{y - \epsilon} {\beta})  & y \geq \epsilon \\
0  & x < \epsilon 
\end{cases}
\end{equation}
```

```{=latex} 
\begin{equation}
f(y; \mu, \beta, \epsilon) = 
\frac{1} {\Gamma(\frac{\mu}{\beta}) \beta^{\frac{\mu}{\beta}}} {(y - \epsilon)}^{\frac{\mu}{\beta} - 1} \exp(- \frac{y - \epsilon} {\beta}) \quad y \geq \epsilon, 
\end{equation}
```